## 1.
$$
\begin{gather}
a(x):=\sum^{\infty}_{k=0}a_{k}(x)^{k} \ \text{mit }|x|<r_{1}\\
b(x):=\sum^{\infty}_{k=0}b_{k}(x)^{k} \ \text{mit }|x|<r_{2}\\ \\
\text{dann folgt: }r:=min\{r_{1},r_{2}\}
\end{gather}

$$

---

## 2.  $a(x)\pm b(x)$
$$
a(x)\pm b(x)=\sum^{\infty}_{k=0}((a_{k}\pm b(x))x^{k} \ \text{für }|x|<r
$$

---

## 3. $c*a(x)$
$$
c*a(x)=\sum^{\infty}_{k=0}(c*a(x))x^{k} \text{ für }|x|<r 
$$
---
## 4. $a(x)*b(x)$ 
$$
a(x)*b(x)=\sum^{\infty}_{k=0}(a_{0}b_{k}+a_{1}b_{k-1}+\dots+a_{k}b_{0})x^{k} \text{ für }|x|<r 
$$

