
#### falls die k-te Ableitung für $f^{(k)}(x_{0})$ existiert für $k=1,2,...$ 

## $$f(x)=p_{n}(x)=\sum^{n}_{k=0} \frac{f^{(k)}(x_{0})}{k!}\cdot(x-x_{0})^{k}$$

---

### Rekursive Definition:
$$
\begin{gather}
p_{0}(x):=f(x_{0})\\
\\
p_{n}(x):=p_{n-1}(x)+ \frac{f^{(n)}(x_{0})}{n!}\cdot(x-x_{0})^{n} \quad (n\geq1)
\end{gather} 

$$
---
# Beispiel

![[WhatsApp Image 2024-05-31 at 10.37.36.jpeg]]

# Es gilt auch:
$$
\begin{gather}
p_{n}(x)=\sum^{n}_{k=0} \frac{f^{(k)}(x_{0})}{k!}\cdot(x-x_{0})^{k} \quad \text{ mit } x_{0}=0\\
=\sum^{n}_{k=0} \frac{f^{(k)}(0)}{k!}\cdot(x)^{k} \\
=\sum^{n}_{k=0} \frac{(-1)^{(k)}(k!)}{k!}\cdot(x)^{k} \\
=\sum^{n}_{k=0} (-1)^{(k)}\cdot(x)^{k} \\
=1-x+x^{2}-x^{3}\dots\pm x^{n}
\end{gather}
$$